continued amendment
Attempt to prove Dijkstra's SSSP according exactly to the description in
CLRS introduction to algorithms

dafny/dijkstra.dfy
@@ -1,6 +1,19 @@
 class Vertex{
   var wfs : int ;         //Vertex contains current length from source as int, does not matter what the type of vertex is
   var pred: int ;        //Vertex Predecessor, "pi" as described in CLRS implementation
+
+  constructor Init()
+  modifies this
+  {
+  this.wfs :=900000;
+  this.pred := 900000;
+  } 
+}
+
+class Edge{
+  var weight : int ;
+  var sourcev : int;
+  var destv : int ;
 }
 
 class Graph{
@@ -10,22 +23,47 @@ class Graph{
   var vertices : array<Vertex>;            //Vertices contained in the graph, since vertices contain the wfs and pred this also 
                                            //contains our shortest paths at the end of the algorithm
 
-  predicate method hasVertex(v: int)
-  reads this;
+  predicate hasVertex(v: int)
+  reads this, this.vertices, this.edgeweights
+  requires this.isValid()
   {
-    0 <= v < size
+    0 <= v < size && 0 <= v < vertices.Length
   }
 
   predicate isValid()
-  requires vertices != null && forall n :: 0 <= n < vertices.Length ==> vertices[n] != null 
-  reads this, this.edgeweights, this.vertices; 
-  reads set m | 0 <= m < this.vertices.Length  :: this.vertices[m]
- // reads set n | 0 <= n < this.edgeweights.Length :: this.edgeweights[n]
+  reads this, this.edgeweights, this.vertices
   {
-   //edgeweights.Length == size &&
-   vertices.Length == size 
-  // forall x :: 0 <= x < edgeweights.Length ==> edgeweights[x].Length == edgeweights.Length &&
-  // forall s, d :: 0  <= s < edgeweights.Length && 0 <= d < edgeweights[s].Length ==>  edgeweights[s][d] > 0
+   (this.edgeweights != null && 
+   this.vertices != null) &&
+   this.edgeweights.Length == size &&
+   this.vertices.Length == size  &&
+   forall n :: 0 <= n < this.vertices.Length ==> this.vertices[n] != null &&
+   forall m :: 0 <= m < this.edgeweights.Length ==> (this.edgeweights[m] != null && this.edgeweights[m].Length == size)
+   /* forall h :: 0 <= h < vertices.Length ==> (vertices[h].wfs != 900000 && vertices[h].pred != 900000) &&
+   forall x :: 0 <= x < edgeweights.Length ==> edgeweights[x].Length == edgeweights.Length  &&
+   forall s, d :: 0  <= s < edgeweights.Length && 0 <= d < edgeweights[s].Length ==>  edgeweights[s][d] > 0 */
+  }
+
+  predicate edges()
+  reads this, this.edgeweights, this.vertices
+  requires this.isValid()
+  reads set m | 0 <= m < edgeweights.Length :: edgeweights[m]
+  {
+  edgeweights != null &&
+  edgeweights.Length == size &&
+  forall n :: 0 <= n < edgeweights.Length ==> edgeweights[n] != null && 
+  edgeweights.Length == edgeweights[n].Length && 
+  edgeweights[n][n] == 0
+  }
+
+  predicate verticesValid()
+  reads this, this.edgeweights, this.vertices
+  requires this.isValid()
+  reads set n | 0 <= n < vertices.Length :: vertices[n]
+  {
+  vertices != null &&
+  vertices.Length == size &&
+  forall n :: 0 <= n < vertices.Length ==> vertices[n] != null 
   }
 }
 
@@ -34,52 +72,68 @@ class Graph{
 
 class MinQueue{
 
-    var Repre : set<int>
+    var Repre : set<Vertex> //representing the queue of vertices using integers
 
-	method Init(capacity: int)
-	modifies this;     //since we always know the queue is never going to be greater capacity than size of graph
+	method Init()  // Initialise queue to have the empty set
+	modifies this;              //since we always know the queue is never going to be greater capacity than size of graph
 	{    
 	 Repre := {};
-	 Repre := Repre + {capacity};
 	}
 
-	method removeMin() returns (vertex: int)
+	method addV(vertex : Vertex)  //add an integer representing a vertex to the queue
 	modifies this;
-	requires Repre != {};
-
 	{
-	  var c:= |Repre|;
-	  var m : int;
-	  var Repres : set<int> := Repre;
-	  while m in Repres
+	  Repre := Repre + {vertex};
+	}
+
+	method removeMin() returns (v: Vertex) // remove the smallest integer from the queue and return it
+	modifies this;                              // since we represent each vertex in the Graph object as its entry in "vertices"
+	requires Repre != {};                       // we need only know which entry has the minimum wfs in the queue
+	{
+	  var c:= 900000;                       // treat 900000 as infinity
+	  var d := 900000;
+	  var m := new Vertex.Init();
+	  v := new Vertex.Init();
+	  var Repres : set<Vertex> := Repre;   //Repres is a copy of the real queue
+
+	  while m in Repres                 //for every integer in Repres( a copy of Repre ), find the minimum 
 	  decreases |Repres| 
 	  {
-	    if m <=c { c := m ;}
+	    if m.wfs <=c { c := m.wfs; d:=m.pred;}
 		Repres := Repres - {m};
 	  }
-	  vertex := c;
-	  Repre := Repre - {vertex};
-	  return vertex;
+	  v.wfs := c;  v.pred := d;   // set the return value to the minimum vertex and remove the found integer from Repre, the real queue
+	  Repre := Repre - {v};
+	  return v;
 	}
    }
 
    class Dijkstra{
 
    method InitializeSS(G : Graph, s: int)
-	 requires G != null && G.isValid() && G.hasVertex(s)
-	 modifies G.vertices 
-	 
+     requires G != null && G.isValid() 
+	 requires G.verticesValid() && G.hasVertex(s)
+	 modifies G, G.vertices
+	 modifies set m | 0 <= m < G.vertices.Length  :: G.vertices[m]
    {
+     assert G.vertices != null;
      var x := G.vertices.Length -1 ;
-	 while x >= 0 {
+     //assert G.vertices != null;
+	 //assert G.hasVertex(s);
+	 while x < G.vertices.Length
+	 invariant G.isValid()
+	 invariant G.verticesValid()
+	 invariant G.hasVertex(s)
+	 {
 	 G.vertices[x].wfs := 900000;
 	 G.vertices[x].pred := 900000;
-     x := x -1 ;
+     x := x + 1 ;
 	 }
+	 //assert G.hasVertex(s);
 	 G.vertices[s].wfs := 0;
    }
 
-   method relax(G: Graph, u: int, v: int, w: int)
+  /* method relax(G: Graph, u: int, v: int, w: int)
     requires G != null && G.isValid() && G.hasVertex(u) && G.hasVertex(v)
 	modifies G.edgeweights
 	//reads G.edgeweights
@@ -89,5 +143,5 @@ class MinQueue{
 	 if G.vertices[v].wfs > G.vertices[u].wfs + G.edgeweights[u][v]
 	 {}
 	 }
-   }
-   }
+   }*/
+   } 
